lib/generic_bv_ops.dfy
@@ -71,6 +71,11 @@ abstract module generic_bv_ops
 
     function method and(x: uint, y: uint): uint
 
+    function method andi(x: uint, imm: sint): uint
+    {
+        and(x, to_2s_comp(imm))
+    }
+
     function method or(x: uint, y: uint): uint
 
     function method not(x: uint) : uint
